Slow progress on Target2.samplePolyCBD.eta3_loop.spec.aux0

proofs/Symcrust/Properties/SamplePolyCBD/Target2SamplePolyCBD.lean
@@ -26,6 +26,7 @@ open Symcrust.Spec
 open Aeneas Aeneas.Std Aeneas.SRRange
 
 set_option maxHeartbeats 1000000
+set_option brute.trust true
 
 structure Target2.samplePolyCBDState where
   η : Η
@@ -185,6 +186,156 @@ lemma Fin.unfold3 {α} [AddCommMonoid α] {n : Nat} (hn : n = 3) (f : Fin n → 
   ∑ x : Fin n, f x = f ⟨0, by omega⟩ + f ⟨1, by omega⟩ + f ⟨2, by omega⟩ := by
   sorry
 
+set_option brute.trust true in
+theorem Target2.samplePolyCBD.eta3_loop.spec.aux0 (s : samplePolyCBDState)
+  (hs1 : ∀ j < s.i, s.pe_dst[j]! = (Target.samplePolyCBD s.B)[j]!) (hs2 : ∀ j < 256, s.i ≤ j → s.pe_dst[j]! = 0)
+  (hs3 : s.src_i * 4 = s.i * 3) (hη : s.η.val = 3) (hs4 : s.i < ↑key.MLWE_POLYNOMIAL_COEFFICIENTS) (j : ℕ)
+  (hj1 : j < s.i + 4) (hj2 : ¬j < s.i)
+  (sample_bits : BitVec (8 * (List.slice s.src_i (s.src_i + 4) s.B.toArray.toList).length))
+  (hsample_bits :
+    sample_bits =
+      (BitVec.fromLEBytes (List.slice s.src_i (s.src_i + 4) s.B.toArray.toList) &&&
+            2396745#(8 * (List.slice s.src_i (s.src_i + 4) s.B.toArray.toList).length)) +
+          (BitVec.fromLEBytes (List.slice s.src_i (s.src_i + 4) s.B.toArray.toList) >>> 1 &&&
+            2396745#(8 * (List.slice s.src_i (s.src_i + 4) s.B.toArray.toList).length)) +
+        (BitVec.fromLEBytes (List.slice s.src_i (s.src_i + 4) s.B.toArray.toList) >>> 2 &&&
+          2396745#(8 * (List.slice s.src_i (s.src_i + 4) s.B.toArray.toList).length)))
+  (hBytesToBits : ∀ i < 64 * s.η.val, ∀ j < 8, (Target.bytesToBits s.B)[8 * i + j]! = s.B[i]!.testBit j)
+  (hj3 : j = s.i) :
+  ((((Vector.set! s.pe_dst s.i ↑↑(inner_loop.next_coefficient s.i 0 (BitVec.setWidth 32 sample_bits)).2).set! (s.i + 1)
+                ↑↑(inner_loop.next_coefficient s.i 1
+                        (inner_loop.next_coefficient s.i 0 (BitVec.setWidth 32 sample_bits)).1).2).set!
+            (s.i + 2)
+            ↑↑(inner_loop.next_coefficient s.i 2
+                    (inner_loop.next_coefficient s.i 1
+                        (inner_loop.next_coefficient s.i 0 (BitVec.setWidth 32 sample_bits)).1).1).2).set!
+        (s.i + 3)
+        ↑↑(inner_loop.next_coefficient s.i 3
+                (inner_loop.next_coefficient s.i 2
+                    (inner_loop.next_coefficient s.i 1
+                        (inner_loop.next_coefficient s.i 0 (BitVec.setWidth 32 sample_bits)).1).1).1).2)[j]! =
+    ∑ (x : Fin s.η.val), ↑(Target.bytesToBits s.B)[2 * j * ↑s.η + ↑x]!.toNat -
+      ∑ (x : Fin s.η.val), ↑(Target.bytesToBits s.B)[2 * j * ↑s.η + ↑s.η + ↑x]!.toNat := by
+  rw [Vector.getElem!_set!_ne (by omega), Vector.getElem!_set!_ne (by omega),
+    Vector.getElem!_set!_ne (by omega), Vector.getElem!_set! (by scalar_tac)]
+  simp only [hj3, hη, Nat.mul_assoc 2 s.i 3, ← hs3, Nat.mul_comm s.src_i 4,
+    ← Nat.mul_assoc 2 4 s.src_i, Nat.reduceMul, Fin.unfold3 hη]
+  specialize hBytesToBits s.src_i (by scalar_tac)
+  rw [hBytesToBits 0 (by omega), hBytesToBits 1 (by omega), hBytesToBits 2 (by omega),
+    hBytesToBits 3 (by omega), hBytesToBits 4 (by omega), Nat.add_assoc,
+    hBytesToBits 5 (by omega)]
+  unfold inner_loop.next_coefficient
+  simp only [BitVec.ofNat_eq_ofNat, ntt.Q.eq, UScalar.ofNat_val_eq, Nat.cast_ofNat,
+    BitVec.toNat_add, BitVec.toNat_sub, Nat.reducePow, BitVec.toNat_ushiftRight,
+    BitVec.toNat_and, BitVec.toNat_setWidth, BitVec.toNat_ofNat, Nat.reduceMod,
+    Nat.mod_add_mod]
+  olet hsample_bits_slice : sample_bits_slice := sample_bits.toNat % 4294967296 &&& 63
+  olet hs_B_byte : s_B_byte := s.B[s.src_i]!
+  replace hs_B_byte : sample_bits_slice = (s_B_byte &&& 9) +
+    ((s_B_byte >>> 1) &&& 9) + ((s_B_byte >>> 2) &&& 9) := by
+    rw [hsample_bits_slice, hsample_bits]
+    simp only [BitVec.toNat_add, BitVec.toNat_and, BitVec.toNat_ofNat,
+      BitVec.toNat_ushiftRight, Nat.mod_add_mod, BitVec.natCast_eq_ofNat, BitVec.ofNat_and,
+      Nat.cast_ofNat, BitVec.ofNat_eq_ofNat]
+    -- Automation note: The automation has a hard time dealing with `min`, hence why I frequently have
+    -- to use `rcases hmin with hmin | hmin <;> (rw [hmin]; ...)` instead of calling a single tactic directly
+    have hmin : min (192 - s.src_i) 4 = 3 ∨ min (192 - s.src_i) 4 = 4 := by scalar_tac
+    simp [List.slice_length, Array.length_toList, Vector.size_toArray,
+      add_tsub_cancel_left, ← BitVec.getElem!_eq_getElem, BitVec.getElem!_and, hη]
+    olet hz : z := (BitVec.fromLEBytes (List.slice s.src_i (s.src_i + 4) s.B.toArray.toList)).toNat >>> 2
+    olet hy : y := (BitVec.fromLEBytes (List.slice s.src_i (s.src_i + 4) s.B.toArray.toList)).toNat >>> 1
+    olet hx : x := (BitVec.fromLEBytes (List.slice s.src_i (s.src_i + 4) s.B.toArray.toList)).toNat
+    olet hx' : x' := (x &&& 2396745 % 2 ^ (8 * min (192 - s.src_i) 4))
+    olet hy' : y' := (y &&& 2396745 % 2 ^ (8 * min (192 - s.src_i) 4))
+    olet hz' : z' := (z &&& 2396745 % 2 ^ (8 * min (192 - s.src_i) 4))
+    rw [Nat.mod_eq_of_lt] at hx' hy' hz' <;> (try rcases hmin with hmin | hmin <;> (rw [hmin]; decide))
+    have hx'' : z' < 2396745 + 1 := by
+      apply Nat.lt_succ_of_le
+      rw [hz']
+      exact Nat.and_le_right
+    have hy'' : y' < 2396745 + 1 := by
+      apply Nat.lt_succ_of_le
+      rw [hy']
+      exact Nat.and_le_right
+    have hz'' : x' < 2396745 + 1 := by
+      apply Nat.lt_succ_of_le
+      rw [hx']
+      exact Nat.and_le_right
+    rw [Nat.mod_eq_of_lt, Nat.mod_eq_of_lt]
+    . rw [(by decide : 63#8 = 2#8^6 - 1#8), BitVec.and_two_pow_sub_one_eq_mod]
+      have : BitVec.ofNat 8 (x' + y' + z') % 2#8 ^ 6 = BitVec.ofNat 8 (x' + y' + z') := by
+        clear hx' hy' hz'; revert x'; revert y'; revert z'; brute
+      rw [this, BitVec.add_def, BitVec.add_def]
+      clear this
+      ext k hk
+      simp only [← BitVec.getElem!_eq_getElem, BitVec.getElem!_eq_testBit_toNat, BitVec.toNat_ofNat,
+        Nat.reducePow, BitVec.toNat_and, Nat.reduceMod, BitVec.toNat_ushiftRight, Nat.mod_add_mod]
+      have : ((x' + y' + z') % 256).testBit k = (x' + y' + z').testBit k := by
+        olet ha : a := x' + y' + z'
+        replace ha : a < 2396746 * 3 := by omega
+        revert a
+        revert k
+        brute
+      rw [this, Nat.mod_eq_of_lt]
+      . rw [hy] at hy'
+        rw [hz] at hz'
+        rw [hx', hy', hz']
+
+        let xBound := x % 2^6
+        have h1 : ∀ k < 8, (xBound &&& 2396745).testBit k = (BitVec.toNat s_B_byte &&& 9).testBit k := by
+          sorry
+        have h2 : ∀ k < 8, ((xBound >>> 1) &&& 2396745).testBit k = (BitVec.toNat s_B_byte &&& 9).testBit k := by
+          sorry
+        have h3 : ∀ k < 8, ((xBound >>> 2) &&& 2396745).testBit k = (BitVec.toNat s_B_byte &&& 9).testBit k := by
+          sorry
+        revert h1 h2 h3
+        clear hx hy hz hx' hy' hz'
+        revert x
+
+        -- Plan: Write a lemma that says if (bottom n bits of a) = (bottom n bits of b) then
+        -- (a + c).testBit k = (b + c).testBit k (so long as `k ≤ n`)
+
+        sorry
+        /-
+        replace hx' : ∀ k < 8, x'.testBit k = (BitVec.toNat s_B_byte &&& 9).testBit k := by
+          intro k hk
+          rw [hx', hx]
+          simp only [Nat.testBit_and]
+          sorry
+        replace hy' : ∀ k < 8, y'.testBit k =
+          ((BitVec.toNat s_B_byte >>> 1) &&& 9).testBit k := by
+          sorry
+        replace hz' : ∀ k < 8, z'.testBit k =
+          ((BitVec.toNat s_B_byte >>> 2) &&& 9).testBit k := by
+          sorry
+        clear this hBytesToBits hs_B_byte
+        revert hx' hy' hz'
+        revert s_B_byte
+        revert z'
+        revert y'
+        revert x'
+        revert k
+        sorry -- brute
+        -/
+      . have : BitVec.toNat s_B_byte &&& 9 ≤ 9 := Nat.and_le_right
+        have : (BitVec.toNat s_B_byte >>> 1) &&& 9 ≤ 9 := Nat.and_le_right
+        have : (BitVec.toNat s_B_byte >>> 2) &&& 9 ≤ 9 := Nat.and_le_right
+        omega
+    . clear hx' hy' hz'
+      revert z'; revert y'; revert x'; rcases hmin with hmin | hmin <;> (rw [hmin]; brute)
+    . clear hx' hy' hz'
+      rw [Nat.mod_eq_of_lt]
+      . revert z'; revert y'; revert x'; brute
+      . revert z'; revert y'; revert x'; rcases hmin with hmin | hmin <;> (rw [hmin]; brute)
+  replace hsample_bits_slice : sample_bits_slice < 64 := by
+    rw [hsample_bits_slice]
+    exact Nat.lt_succ_of_le Nat.and_le_right
+  clear hBytesToBits
+  revert s_B_byte
+  revert sample_bits_slice
+  brute
+
+/-
 def Target2.samplePolyCBD.eta3_loop.spec {η : Η} (s : Target2.samplePolyCBDState)
   (hs1 : ∀ j < s.i, s.pe_dst[j]! = (Target.samplePolyCBD s.B)[j]!)
   (hs2 : ∀ j < 256, s.i ≤ j → s.pe_dst[j]! = 0)
@@ -210,44 +361,16 @@ def Target2.samplePolyCBD.eta3_loop.spec {η : Η} (s : Target2.samplePolyCBDSta
                 2396745#(8 * (List.slice s.src_i (s.src_i + 4) s.B.toArray.toList).length)) +
             (BitVec.fromLEBytes (List.slice s.src_i (s.src_i + 4) s.B.toArray.toList) >>> 2 &&&
               2396745#(8 * (List.slice s.src_i (s.src_i + 4) s.B.toArray.toList).length)))
-        have j_upper_bound : j < 256 := by
-          -- `s.i + 4 ≤ 256` because `s.i < 256` (from `hs4`) and `4 ∣ s.i` from `hs3`
-          -- Since `j < s.i + 4` (from `hj1`) it follows that `j < 256` as desired
-          sorry
-        rw [Target.samplePolyCBD.spec s.B j (by omega), ← Symcrust.SpecAux.Target.bytesToBits.eq_spec]
+        rw [Target.samplePolyCBD.spec s.B j (by scalar_tac), ← Symcrust.SpecAux.Target.bytesToBits.eq_spec]
         have hBytesToBits := Target.bytesToBits.spec s.B
         unfold Target.bytesToBits.post at hBytesToBits
         unfold inner_loop
         simp only [Q, Vector.Inhabited_getElem_eq_getElem!, Nat.cast_sum]
         have hj3 : j = s.i ∨ j = s.i + 1 ∨ j = s.i + 2 ∨ j = s.i + 3 := by omega
         rcases hj3 with hj3 | hj3 | hj3 | hj3
+        . apply eta3_loop.spec.aux0 <;> assumption
         . rw [Vector.getElem!_set!_ne (by omega), Vector.getElem!_set!_ne (by omega),
-            Vector.getElem!_set!_ne (by omega), Vector.getElem!_set! (by omega)]
-          simp only [hj3, hη, Nat.mul_assoc 2 s.i 3, ← hs3, Nat.mul_comm s.src_i 4,
-            ← Nat.mul_assoc 2 4 s.src_i, Nat.reduceMul, Fin.unfold3 hη]
-          specialize hBytesToBits s.src_i (by omega)
-          rw [hBytesToBits 0 (by omega), hBytesToBits 1 (by omega), hBytesToBits 2 (by omega),
-            hBytesToBits 3 (by omega), hBytesToBits 4 (by omega), Nat.add_assoc,
-            hBytesToBits 5 (by omega)]
-          unfold inner_loop.next_coefficient
-          simp only [BitVec.ofNat_eq_ofNat, ntt.Q.eq, UScalar.ofNat_val_eq, Nat.cast_ofNat,
-            BitVec.toNat_add, BitVec.toNat_sub, Nat.reducePow, BitVec.toNat_ushiftRight,
-            BitVec.toNat_and, BitVec.toNat_setWidth, BitVec.toNat_ofNat, Nat.reduceMod,
-            Nat.mod_add_mod]
-          olet hsample_bits_slice : sample_bits_slice := sample_bits.toNat % 4294967296 &&& 63
-          olet hs_B_byte : s_B_byte := s.B[s.src_i]!
-          replace hs_B_byte : sample_bits_slice = (s_B_byte &&& 9) +
-            ((s_B_byte >>> 1) &&& 9) + ((s_B_byte >>> 2) &&& 9) := by
-            sorry
-          replace hsample_bits_slice : sample_bits_slice < 64 := by
-            rw [hsample_bits_slice]
-            exact Nat.lt_succ_of_le Nat.and_le_right
-          clear hBytesToBits
-          revert s_B_byte
-          revert sample_bits_slice
-          brute
-        . rw [Vector.getElem!_set!_ne (by omega), Vector.getElem!_set!_ne (by omega),
-            Vector.getElem!_set! (by omega)]
+            Vector.getElem!_set! (by scalar_tac)]
           simp only [hj3, hη, Nat.mul_assoc 2 (s.i + 1) 3, Nat.mul_comm (s.i + 1) 3,
             Nat.mul_add 3 s.i 1, Nat.mul_comm 3 s.i, ← hs3, Nat.mul_comm s.src_i 4, mul_one,
             Nat.mul_add 2 (4 * s.src_i) 3, ← Nat.mul_assoc 2 4 s.src_i, Nat.reduceMul,
@@ -256,12 +379,12 @@ def Target2.samplePolyCBD.eta3_loop.spec {η : Η} (s : Target2.samplePolyCBDSta
           conv in 8 * s.src_i + 9 => rw [(by omega : 8 * s.src_i + 9 = 8 * (s.src_i + 1) + 1)]
           conv in 8 * s.src_i + 10 => rw [(by omega : 8 * s.src_i + 10 = 8 * (s.src_i + 1) + 2)]
           conv in 8 * s.src_i + 11 => rw [(by omega : 8 * s.src_i + 11 = 8 * (s.src_i + 1) + 3)]
-          rw [hBytesToBits s.src_i (by omega) 6 (by omega),
-              hBytesToBits s.src_i (by omega) 7 (by omega),
-              hBytesToBits (s.src_i + 1) (by omega) 0 (by omega),
-              hBytesToBits (s.src_i + 1) (by omega) 1 (by omega),
-              hBytesToBits (s.src_i + 1) (by omega) 2 (by omega),
-              hBytesToBits (s.src_i + 1) (by omega) 3 (by omega)]
+          rw [hBytesToBits s.src_i (by scalar_tac) 6 (by omega),
+              hBytesToBits s.src_i (by scalar_tac) 7 (by omega),
+              hBytesToBits (s.src_i + 1) (by scalar_tac) 0 (by omega),
+              hBytesToBits (s.src_i + 1) (by scalar_tac) 1 (by omega),
+              hBytesToBits (s.src_i + 1) (by scalar_tac) 2 (by omega),
+              hBytesToBits (s.src_i + 1) (by scalar_tac) 3 (by omega)]
           unfold inner_loop.next_coefficient
           simp only [BitVec.ofNat_eq_ofNat, ntt.Q.eq, UScalar.ofNat_val_eq, Nat.cast_ofNat,
             BitVec.toNat_add, BitVec.toNat_sub, Nat.reducePow, BitVec.toNat_ushiftRight,
@@ -283,7 +406,7 @@ def Target2.samplePolyCBD.eta3_loop.spec {η : Η} (s : Target2.samplePolyCBDSta
           revert sample_bits_slice
           -- Once I finish the statements of `hs_B_byte0` and `hs_B_byte1` this should be provable via `brute`
           sorry
-        . rw [Vector.getElem!_set!_ne (by omega), Vector.getElem!_set! (by omega)]
+        . rw [Vector.getElem!_set!_ne (by omega), Vector.getElem!_set! (by scalar_tac)]
           simp only [hj3, hη, Nat.mul_assoc 2 (s.i + 2) 3, Nat.mul_comm (s.i + 2) 3,
             Nat.mul_add 3 s.i 2, Nat.mul_comm 3 s.i, ← hs3, Nat.mul_comm s.src_i 4, mul_one,
             Nat.mul_add 2 (4 * s.src_i) 6, ← Nat.mul_assoc 2 4 s.src_i, Nat.reduceMul,
@@ -294,12 +417,12 @@ def Target2.samplePolyCBD.eta3_loop.spec {η : Η} (s : Target2.samplePolyCBDSta
           conv in 8 * s.src_i + 15 => rw [(by omega : 8 * s.src_i + 15 = 8 * (s.src_i + 1) + 7)]
           conv in 8 * s.src_i + 16 => rw [(by omega : 8 * s.src_i + 16 = 8 * (s.src_i + 2) + 0)]
           conv in 8 * s.src_i + 17 => rw [(by omega : 8 * s.src_i + 17 = 8 * (s.src_i + 2) + 1)]
-          rw [hBytesToBits (s.src_i + 1) (by omega) 4 (by omega),
-              hBytesToBits (s.src_i + 1) (by omega) 5 (by omega),
-              hBytesToBits (s.src_i + 1) (by omega) 6 (by omega),
-              hBytesToBits (s.src_i + 1) (by omega) 7 (by omega),
-              hBytesToBits (s.src_i + 2) (by omega) 0 (by omega),
-              hBytesToBits (s.src_i + 2) (by omega) 1 (by omega)]
+          rw [hBytesToBits (s.src_i + 1) (by scalar_tac) 4 (by omega),
+              hBytesToBits (s.src_i + 1) (by scalar_tac) 5 (by omega),
+              hBytesToBits (s.src_i + 1) (by scalar_tac) 6 (by omega),
+              hBytesToBits (s.src_i + 1) (by scalar_tac) 7 (by omega),
+              hBytesToBits (s.src_i + 2) (by scalar_tac) 0 (by omega),
+              hBytesToBits (s.src_i + 2) (by scalar_tac) 1 (by omega)]
           unfold inner_loop.next_coefficient
           simp only [BitVec.ofNat_eq_ofNat, ntt.Q.eq, UScalar.ofNat_val_eq, Nat.cast_ofNat,
             BitVec.toNat_add, BitVec.toNat_sub, Nat.reducePow, BitVec.toNat_ushiftRight,
@@ -322,7 +445,7 @@ def Target2.samplePolyCBD.eta3_loop.spec {η : Η} (s : Target2.samplePolyCBDSta
           revert sample_bits_slice
           -- Once I finish the statements of `hs_B_byte1` and `hs_B_byte2` this should be provable via `brute`
           sorry
-        . rw [Vector.getElem!_set! (by omega)]
+        . rw [Vector.getElem!_set! (by scalar_tac)]
           simp only [hj3, hη, Nat.mul_assoc 2 (s.i + 3) 3, Nat.mul_comm (s.i + 3) 3,
             Nat.mul_add 3 s.i 3, Nat.mul_comm 3 s.i, ← hs3, Nat.mul_comm s.src_i 4, mul_one,
             Nat.mul_add 2 (4 * s.src_i) 9, ← Nat.mul_assoc 2 4 s.src_i, Nat.reduceMul,
@@ -333,12 +456,12 @@ def Target2.samplePolyCBD.eta3_loop.spec {η : Η} (s : Target2.samplePolyCBDSta
           conv in 8 * s.src_i + 21 => rw [(by omega : 8 * s.src_i + 21 = 8 * (s.src_i + 2) + 5)]
           conv in 8 * s.src_i + 22 => rw [(by omega : 8 * s.src_i + 22 = 8 * (s.src_i + 2) + 6)]
           conv in 8 * s.src_i + 23 => rw [(by omega : 8 * s.src_i + 23 = 8 * (s.src_i + 2) + 7)]
-          rw [hBytesToBits (s.src_i + 2) (by omega) 2 (by omega),
-              hBytesToBits (s.src_i + 2) (by omega) 3 (by omega),
-              hBytesToBits (s.src_i + 2) (by omega) 4 (by omega),
-              hBytesToBits (s.src_i + 2) (by omega) 5 (by omega),
-              hBytesToBits (s.src_i + 2) (by omega) 6 (by omega),
-              hBytesToBits (s.src_i + 2) (by omega) 7 (by omega)]
+          rw [hBytesToBits (s.src_i + 2) (by scalar_tac) 2 (by omega),
+              hBytesToBits (s.src_i + 2) (by scalar_tac) 3 (by omega),
+              hBytesToBits (s.src_i + 2) (by scalar_tac) 4 (by omega),
+              hBytesToBits (s.src_i + 2) (by scalar_tac) 5 (by omega),
+              hBytesToBits (s.src_i + 2) (by scalar_tac) 6 (by omega),
+              hBytesToBits (s.src_i + 2) (by scalar_tac) 7 (by omega)]
           unfold inner_loop.next_coefficient
           simp only [BitVec.ofNat_eq_ofNat, ntt.Q.eq, UScalar.ofNat_val_eq, Nat.cast_ofNat,
             BitVec.toNat_add, BitVec.toNat_sub, Nat.reducePow, BitVec.toNat_ushiftRight,
@@ -395,5 +518,6 @@ def Target2.samplePolyCBD.spec {η : Η} (B : Vector Byte (64 * η)) : samplePol
       simp only [Set.instMembership, Set.Mem, insert, Set.insert, setOf, singleton, Set.singleton] at hη
       omega
     apply eta2_loop.spec <;> assumption
+-/
 
 end Symcrust.SpecAux
